theories/LogicalRelation/Introductions/Application.v
@@ -11,57 +11,58 @@ Smpl Add fold_subst_term : refold.
 Section Application.
 Context `{GenericTypingProperties}.
 
-Lemma ScodSubst {Γ u u' F F' G G' l l'}
+Lemma ScodSubst {Γ} {wfΓ : [|-Γ]} {u u' F F' G G' l l'}
   (RΠ : [Γ ||-S<l> tProd F G ≅ tProd F' G'])
   {RF : [Γ ||-S<l'> F ≅ F']}
   (Ruu' : [Γ ||-S<l'> u ≅ u' : F | RF ]) :
-  [Γ ||-<l> G[u..] ≅ G'[u'..]].
+  [wfΓ ||-<l> G[u..] ≅ G'[u'..]].
 Proof.
   set (RΠ' :=normRedΠ RΠ).
-  eapply instKripkeSubst, SirrLR, Ruu'. shelve.
+  eapply instKripkeSubst, SirrLR, Ruu'.
   intros; eapply RΠ'.(PolyRed.posRed); eapply SirrLR, hab.
   Unshelve.
-  3: eapply instKripke.
+  3: eapply SinstKripke.
   2,4: eapply RΠ'.(PolyRed.shpRed).
-  3: tea.
-  all: escape; gtyping.
+  easy.
 Qed.
 
-Lemma codSubst {Γ u u' F F' G G' l l'}
-  (RΠ : [Γ ||-<l> tProd F G ≅ tProd F' G'])
-  {RF : [Γ ||-<l'> F ≅ F']}
-  (Ruu' : [Γ ||-<l'> u ≅ u' : F | RF ]) :
-  [Γ ||-<l> G[u..] ≅ G'[u'..]].
+Lemma codSubst {Γ} {wfΓ : [|-Γ]} {u u' F F' G G' l l'}
+  (RΠ : [wfΓ ||-<l> tProd F G ≅ tProd F' G'])
+  {RF : [wfΓ ||-<l'> F ≅ F']}
+  (Ruu' : [wfΓ ||-<l'> u ≅ u' : F | RF ]) :
+  [wfΓ ||-<l> G[u..] ≅ G'[u'..]].
 Proof.
-  eapply (dSplit_bind_over Ruu').
-  intros Δ ρ oRF oRuu'.
-  eapply WrePack, (Split_wk_bind_over RΠ ρ).
-  intros Ξ ρΞ oRΠ.
-  eapply WrePack.
+  eapply (dSplit_bind Ruu').
+  intros Δ wfΔ ρ oRF oRuu'.
+  eapply WAdrefold, (Split_wk_bind RΠ ρ).
+  intros Ξ wfΞ ρΞ oRΠ.
+  eapply WAdrefold.
   erewrite 2!wk_comp_ren_on.
   erewrite 2!(subst_ren_wk_up).
-  eapply ScodSubst, Ruu', overtree_PSh, oRuu'.
-  eapply RΠ.
+  unshelve eapply ScodSubst, Ruu'.
+  3: now eapply RΠ. Unshelve.
+  easy. 1,2: now eapply overtree_PSh.
+  apply F. apply F'.
+Qed.
 
-Lemma appcongTerm {Γ t t' u u' F F' G G' l l'}
-  (RΠ : [Γ ||-<l> tProd F G ≅ tProd F' G'])
-  {RF : [Γ ||-<l'> F ≅ F']}
-  (Rtt' : [Γ ||-<l> t ≅ t' : tProd F G | RΠ])
-  (Ruu' : [Γ ||-<l'> u ≅ u' : F | RF ])
-  (RGu : [Γ ||-<l'> G[u..] ≅ G'[u'..]]) :
-    [Γ ||-<l'> tApp t u ≅ tApp t' u' : G[u..] | RGu].
+Lemma appcongTerm {Γ} {wfΓ : [|-Γ]} {t t' u u' F F' G G' l l'}
+  (RΠ : [Γ ||-S<l> tProd F G ≅ tProd F' G'])
+  {RF : [Γ ||-S<l'> F ≅ F']}
+  (Rtt' : [Γ ||-S<l> t ≅ t' : tProd F G | RΠ])
+  (Ruu' : [Γ ||-S<l'> u ≅ u' : F | RF ])
+  (RGu : [wfΓ ||-<l'> G[u..] ≅ G'[u'..]]) :
+    [wfΓ ||-<l'> tApp t u ≅ tApp t' u' : G[u..] | RGu].
 Proof.
   set (RΠ' :=normRedΠ RΠ).
-  assert [LRPi' RΠ' | _ ||- t ≅ t' : _ ] as [Rt Rt' ? app] by now eapply irrLREq.
-  assert (wfΓ : [|-Γ]) by (escape ; gtyping).
+  assert [LRPi' RΠ' | _ ||- t ≅ t' : _ ] as [Rt Rt' ? app] by now eapply SirrLREq.
   eapply redSubstTmEq.
-(*   + unshelve (eapply irrLREqCum, app; cbn; now erewrite eq_subst_scons); [|tea|].
-    2: rewrite wk_id_ren_on; eapply irrLREqCum; tea; now rewrite wk_id_ren_on.
+  + unshelve (eapply irrLREqCum, app; cbn; now erewrite eq_subst_scons).
+    2: rewrite wk_id_ren_on; eapply SirrLREqCum; tea; now rewrite wk_id_ren_on.
   + rewrite 2!wk_id_ren_on; eapply redtm_app; [now destruct (PiRedTmEq.red Rt)| now escape].
   + rewrite wk_id_ren_on; eapply redtm_app.
     2: eapply ty_conv; now escape.
-    1: eapply redtm_conv; [now destruct (PiRedTmEq.red Rt')| now escape]. *)
-Admitted.
+    1: eapply redtm_conv; [now destruct (PiRedTmEq.red Rt')| now escape].
+Qed.
 
 End Application.
 
